wip: Looking at destruct_fs_beh

rupicola/io/IO.fst
@@ -434,6 +434,7 @@ let destruct_fs_beh_read #t1 #t2 (args:io_args ORead) (res:io_res ORead args) (c
   end
 *)
 
+(*
 let rec extend_theta_to_io_bind #t1 #t2 (m:io t1) (f:t1 -> io t2) (h:history) (p:hist_post h t1) :
   Lemma (requires (theta m h p))
         (ensures  (exists lt1 fs_m . theta (io_bind m f) h (fun lt _ -> exists (lt2: local_trace (h ++ lt1)) . lt = lt1@lt2 /\ p lt1 fs_m))) =
@@ -451,16 +452,21 @@ let rec extend_theta_to_io_bind #t1 #t2 (m:io t1) (f:t1 -> io t2) (h:history) (p
     assert (hist_bind (op_wp o args) (fun r -> theta (k r)) h p);
     assert ((op_wp o args) h (fun lt r ->  theta (k r) (h ++ lt) (fun lt' r' -> p (lt @ lt') r')));
     admit ()
+*)
 
-let destruct_fs_beh' #t1 #t2 (m:io t1) (k:t1 -> io t2) (h:history) (lt:local_trace h) (fs_r:t2) :
-  Lemma
-    (requires thetaP (io_bind m k) h lt fs_r) // forall p. theta (io_bind m k) h p ==> p lt fs_r
-    (ensures exists (lt1:local_trace h) (lt2:local_trace (h++lt1)) (fs_m:t1).
-      lt == (lt1@lt2) /\
-      thetaP m h lt1 fs_m) = // forall p. theta m h p ==> p lt1 fs_m
-  assert (forall (p:hist_post h t2). theta (io_bind m k) h p ==> p lt fs_r);
-  admit ()
+unfold
+let theta_io_bind_exists_post #t1 #t2 (m:io t1) (f:t1 -> io t2) (h:history) (lt:local_trace h) (fs_r:t2) =
+  exists fs_m lt1 lt2 . 
+      lt = lt1@lt2 /\ 
+      thetaP m h lt1 fs_m /\
+      thetaP (f fs_m) (h++lt1) lt2 fs_r
 
+let rec theta_io_bind_exists #t1 #t2 (m:io t1) (f:t1 -> io t2) (h:history) : Lemma (theta (io_bind m f) h (theta_io_bind_exists_post m f h)) =
+  match m with
+  | Return x ->
+      assume (theta (f x) h (fun lt fs_r -> 
+        exists fs_m lt1 lt2 . lt = lt1@lt2 /\ thetaP (Return x) h lt1 fs_m /\ thetaP (f fs_m) (h++lt1) lt2 fs_r))
+  | Call o args k -> admit ()
 
 let destruct_fs_beh #t1 #t2 (m:io t1) (k:t1 -> io t2) (h:history) (lt:local_trace h) (fs_r:t2) :
   Lemma
